@prefix hm: <http://vocab.cosmicdynamo.net/hypermedia.owl#> .
@prefix doc: <http://vocab.cosmicdynamo.net/documentation.owl#> .

@prefix dc: <http://purl.org/dc/elements/1.1/> .
@prefix owl: <http://www.w3.org/2002/07/owl#> .
@prefix rdf: <http://www.w3.org/1999/02/22-rdf-syntax-ns#> .
@prefix xml: <http://www.w3.org/XML/1998/namespace> .
@prefix xsd: <http://www.w3.org/2001/XMLSchema#> .
@prefix http: <http://www.w3.org/2011/http#> .
@prefix rdfs: <http://www.w3.org/2000/01/rdf-schema#> .
@prefix schema: <http://schema.org/> .

@base <http://vocab.cosmicdynamo.net/hypermedia.owl> .

<http://vocab.cosmicdynamo.net/hypermedia.owl> rdf:type owl:Ontology ;
    rdfs:label "Hypermedia Ontology" ;
    owl:versionInfo "draft"^^xsd:string ;
    dc:dateSubmitted "2014-12-06"^^xsd:date ;
    dc:creator <mailto:bpease@cosmicdynamo.net> ;
    dc:publisher <http://cosmicdynamo.net> ;
    rdfs:comment """Describes the interface by which a Semantic Agent can interact with a RESTful Semantic Service"""" ;
    <http://purl.org/vocab/vann/preferredNamespacePrefix> "hm"  ;
    <http://purl.org/vocab/vann/preferredNamespaceUri> "http://vocab.cosmicdynamo.net/hypermedia.owl#" .


#################################################################
#
#    Object Properties
#
#################################################################

###  http://vocab.cosmicdynamo.net/hypermedia.owl#acceptsResource
hm:acceptsResource a owl:ObjectProperty ;
  rdfs:label "Accepts Resource" ;
  rdfs:comment "If this property is provided then any requests to the server MUST have a body with an object of the acceptable Resource type" ;
  rdfs:domain hm:HypermediaLink ;
  rdfs:range owl:Class  ;
  doc:example """
    @prefix hm: <http://vocab.cosmicdynamo.net/hypermedia.owl#> .
    @prefix ex: <http://example.com/example.owl#> .

    @base <http://example.com/> .

    <Object/initial> a hm:Resource ;
      hm:hasLink [ 
        a hm:IdempotentLink ,
          ex:Action ;
        hm:hasMethod hm:Put ;
        hm:url "http://example.com/Object" ;
        hm:acceptsResource ex:ObjectType
      ] .
  """ .

###  http://vocab.cosmicdynamo.net/hypermedia.owl#dataPredicate
hm:dataPredicate a owl:ObjectProperty ;
  rdfs:label "Data Predicate" ;
  rdfs:comment "This property is used on the Source Data link to inform the consumer what property on the parent object this link provides data for." ;
  rdfs:domain hm:SourceDataLink ;
  rdfs:range rdf:Property ;
  doc:example """
    @prefix hm: <http://vocab.cosmicdynamo.net/hypermedia.owl#> .
    @prefix ex: <http://example.com/example.owl#> .

    @base <http://example.com/> .

    <Object/initial> a hm:Resource ;
      ex:hasField <Enumeration/000> ;
      hm:hasLink [ 
        a hm:IdempotentLink ,
          hm:SourceDataLink ;
        hm:hasMethod hm:Get ;
        hm:url "http://example.com/Enumeration" ;
        hm:providesResource ex:EnumeratedType ;
        hm:dataPredicate ex:hasField
      ] .
  """ .


###  http://vocab.cosmicdynamo.net/hypermedia.owl#hasLink
hm:hasLink a owl:ObjectProperty ;
  rdfs:label "Links" ;
  rdfs:comment "The collection of RESTful Hypermedia actions that can be performed on a given object" ;
  rdfs:domain hm:Resource ;
  rdfs:range hm:HypermediaLink ;
  doc:example """
    @prefix hm: <http://vocab.cosmicdynamo.net/hypermedia.owl#> .
    @prefix ex: <http://example.com/example.owl#> .

    @base <http://example.com/> .

    <Object/id/0> a hm:Resource ;
      hm:hasLink  [ 
        a hm:IdempotentLink ,
          ex:Action ;
        hm:hasMethod hm:Put ;
        hm:url "http://example.com/Object/doSomething" ;
      ] .
  """ .

###  http://vocab.cosmicdynamo.net/hypermedia.owl#hasMethod
hm:hasMethod a owl:ObjectProperty ;
  rdfs:label "Method" ;
  rdfs:comment "The HTTP method to use when executing this Hypermedia Link" ;
  rdfs:domain hm:HypermediaLink ;
  rdfs:range hm:HttpMethod ;
  doc:example """
    @prefix hm: <http://vocab.cosmicdynamo.net/hypermedia.owl#> .
    @prefix ex: <http://example.com/example.owl#> .

    @base <http://example.com/> .

    <Object/id/0> a hm:Resource ;
      hm:hasLink  [ 
        a hm:IdempotentLink ,
          ex:Action ;
        hm:hasMethod hm:Put ;
        hm:url "http://example.com/Object/doSomething" ;
      ] .
  """ .

###  http://vocab.cosmicdynamo.net/hypermedia.owl#hasOntology
hm:hasOntology a owl:ObjectProperty ;
  rdfs:label "Ontology" ;
  rdfs:comment "Link to a subset of an OWL ontology which describes the owl:class served by this hypermedia resource" ;
  rdfs:domain hm:ResourceDescription ;
  rdfs:range owl:Ontology ;
  doc:example """
    @prefix hm: <http://vocab.cosmicdynamo.net/hypermedia.owl#> .
    @prefix col: <http://vocab.cosmicdynamo.net/collection.owl#> .
    @prefix ex: <http://example.com/example.owl#> .
    
    @prefix xsd: <http://www.w3.org/2001/XMLSchema#> .

    @base <http://example.com/api/> .

    <?objectType=http%3A%2F%2Fexample.com%2F2014%2Fexample.owl%23ObjectType> a hm:ResourceDiscoveryDocument;
      hm:hasResource ( <ObjectType> ) .
                  
    <ObjectType/Resources> a col:Container ;
      col:membershipSubject <?objectType=http%3A%2F%2Fexample.com%2F2014%2Fexample.owl%23ObjectType> ;
      col:membershipPredicate hm:hasResource ;
      col:totalCount "1"^^xsd:nonNegativeInteger .

    <ObjectType> a hm:ResourceDescription ;
      hm:hasOntology <ObjectType/ontology> ;
      hm:serves ex:ObjectType .
  """ .

###  http://vocab.cosmicdynamo.net/hypermedia.owl#hasTemplateItem
hm:hasTemplateItem a owl:ObjectProperty ;
  rdfs:label "Template Item List" ;
  rdfs:comment "List of template item(s) describing valid parameters used to form the URL for this Hypermedia Link" ;
  rdfs:domain hm:TemplateLink ;
  rdfs:range hm:TemplateItem ;
  doc:example """
    @prefix hm: <http://vocab.cosmicdynamo.net/hypermedia.owl#> .
    @prefix ex: <http://example.com/example.owl#> .
    
    <Object/id/1> a hm:Resource ;
      ex:field "value" ;
      hm:hasLink [
        a hm:TemplateLink ,
          ex:Action ;
        hm:templateUrl "http://example.com/Object/id/1/doSomething?param={value}" ;
        hm:hasMethod hm:Put ;
        hm:hasTemplateItem [
          hm:token "{value}" ;
          hm:templateItemPredicate ex:field 
        ]
      ] .
  """ .

###  http://vocab.cosmicdynamo.net/hypermedia.owl#providesResource
hm:providesResource a owl:ObjectProperty ;
  rdfs:label "Provides Resource" ;
  rdfs:comment "Informs the consumer what Object Type is contained in the response body for this link." ;
  rdfs:domain hm:HypermediaLink ;
  rdfs:range owl:Class ;
  doc:example """
    @prefix hm: <http://vocab.cosmicdynamo.net/hypermedia.owl#> .
    @prefix ex: <http://example.com/example.owl#> .
    
    @base <http://example.com/> .

    <Object/id/0> a hm:Resource ;
      hm:hasLink  [ 
        a hm:IdempotentLink ,
          ex:Action ;
        hm:hasMethod hm:Get ;
        hm:url "http://example.com/Object/details" ;
        hm:providesResource ex:ChildThing
      ] .
  """ .

###  http://vocab.cosmicdynamo.net/hypermedia.owl#templateItemPredicate
hm:templateItemPredicate a owl:ObjectProperty ;
  rdfs:label "Template-Item Predicate" ;
  rdfs:comment "This predicate is used in combination with the hm:token to take the string value of the object and replace the token identified in the template url." ;
  rdfs:domain hm:TemplateItem ;
  rdfs:range rdf:Property ;
  doc:example """
    @prefix hm: <http://vocab.cosmicdynamo.net/hypermedia.owl#> .
    @prefix ex: <http://example.com/example.owl#> .
    
    <Object/id/1> a hm:Resource ;
      ex:field "value" ;
      hm:hasLink [
        a hm:TemplateLink ,
          ex:Action ;
        hm:templateUrl "http://example.com/Object/id/1/doSomething?param={value}" ;
        hm:hasMethod hm:Put ;
        hm:hasTemplateItem [
          hm:token "{value}" ;
          hm:templateItemPredicate ex:field 
        ]
      ] .
  """ .


###  http://vocab.cosmicdynamo.net/hypermedia.owl#hasResource
hm:hasResource a owl:ObjectProperty ;
  rdfs:label "Has Resource" ;
  rdfs:comment "List of resources that are available under the current resource search" ;
  rdfs:domain hm:ResourceDiscoveryDocument ;
  rdfs:range hm:ResourceDescription ;
  doc:example """
    @prefix hm: <http://vocab.cosmicdynamo.net/hypermedia.owl#> .
    @prefix col: <http://vocab.cosmicdynamo.net/collection.owl#> .
    @prefix ex: <http://example.com/example.owl#> .

    @prefix xsd: <http://www.w3.org/2001/XMLSchema#> .

    @base <http://example.com/api/> .

    <?objectType=http%3A%2F%2Fexample.com%2F2014%2Fexample.owl%23ObjectType> a hm:ResourceDiscoveryDocument;
      hm:hasResource ( <ObjectType> ) .
                  
    <ObjectType/Resources> a col:Container ;
      col:membershipSubject <?objectType=http%3A%2F%2Fexample.com%2F2014%2Fexample.owl%23ObjectType> ;
      col:membershipPredicate hm:hasResource ;
      col:totalCount "1"^^xsd:nonNegativeInteger.

    <ObjectType> a hm:ResourceDescription ;
      hm:hasOntology <ObjectType/ontology> ;
      hm:serves ex:ObjectType .
  """ .

###  http://vocab.cosmicdynamo.net/hypermedia.owl#serves
hm:serves a owl:ObjectProperty ;
  rdfs:label "Serves" ;
  rdfs:comment "Information on what Object Type a given resource definition provides details about" ;
  rdfs:domain hm:ResourceDescription ;
  rdfs:range owl:Class ;
  doc:example """
    @prefix hm: <http://vocab.cosmicdynamo.net/hypermedia.owl#> .
    @prefix col: <http://vocab.cosmicdynamo.net/collection.owl#> .
    @prefix ex: <http://example.com/example.owl#> .
    
    @prefix xsd: <http://www.w3.org/2001/XMLSchema#> .

    @base <http://example.com/api/> .

    <?objectType=http%3A%2F%2Fexample.com%2F2014%2Fexample.owl%23ObjectType> a hm:ResourceDiscoveryDocument;
      hm:hasResource ( <ObjectType> ) .
                  
    <ObjectType/Resources> a col:Container ;
      col:membershipSubject <?objectType=http%3A%2F%2Fexample.com%2F2014%2Fexample.owl%23ObjectType> ;
      col:membershipPredicate hm:hasResource ;
      col:totalCount "1"^^xsd:nonNegativeInteger .

    <ObjectType> a hm:ResourceDescription ;
      hm:hasOntology <ObjectType/ontology> ;
      hm:serves ex:ObjectType .
  """ .

### http://vocab.cosmicdynamo.net/hypermedia.owl#useFrame
hm:useFrame a owl:ObjectProperty ;
  rdfs:domain hm:HypermediaLink ;
  rdfs:range hm:Frame ;
  rdfs:label "Use Frame" ;
  rdfs:comment "Framing information to reduce the request data to only information the server can handle" ;
  doc:example """
    @prefix hm: <http://vocab.cosmicdynamo.net/hypermedia.owl#> .
    @prefix ex: <http://example.com/example.owl#> .
    
    @base <http://example.com/> .

    <Object/initial> a hm:Resource ;
    hm:hasLink [ 
      a hm:IdempotentLink ,
        ex:Action ;
      hm:hasMethod hm:Put ;
      hm:url "http://example.com/Object" ;
      hm:acceptsResource ex:NonPersonalClient ;
      hm:useFrame <ObjectType/frame> 
    ] .
  """ .
                

#################################################################
#
#    Data properties
#
#################################################################

###  http://vocab.cosmicdynamo.net/hypermedia.owl#templateUrl
hm:templateUrl a owl:DatatypeProperty ;
  rdfs:label "Template URL" ;
  rdfs:comment "A string with replacement tags that enable the dynamic, data-driven, construction of a request URL" ;
  rdfs:domain hm:TemplateLink ;
  rdfs:range xsd:string ;
  doc:example """
    @prefix hm: <http://vocab.cosmicdynamo.net/hypermedia.owl#> .
    @prefix ex: <http://example.com/example.owl#> .
    
    <Object/id/1> a hm:Resource ;
      ex:field "value" ;
      hm:hasLink [
        a hm:TemplateLink ,
          ex:Action ;
        hm:templateUrl "http://example.com/Object/id/1/doSomething?param={value}" ;
        hm:hasMethod hm:Put ;
        hm:hasTemplateItem [
          hm:token "{value}" ;
          hm:templateItemPredicate ex:field 
        ]
      ] .
  """ .

###  http://vocab.cosmicdynamo.net/hypermedia.owl#token
hm:token a owl:DatatypeProperty ;
  rdfs:label "Token" ;
  rdfs:comment "Token in a string to be replaced out at runtime by some value" ;
  rdfs:domain hm:TemplateItem ;
  rdfs:range xsd:string ;
  doc:example """
    @prefix hm: <http://vocab.cosmicdynamo.net/hypermedia.owl#> .
    @prefix ex: <http://example.com/example.owl#> .
    
    <Object/id/1> a hm:Resource ;
      ex:field "value" ;
      hm:hasLink [
        a hm:TemplateLink ,
          ex:Action ;
        hm:templateUrl "http://example.com/Object/id/1/doSomething?param={value}" ;
        hm:hasMethod hm:Put ;
        hm:hasTemplateItem [
          hm:token "{value}" ;
          hm:templateItemPredicate ex:field 
        ]
      ] .
  """ .

###  http://vocab.cosmicdynamo.net/hypermedia.owl#url
hm:url a owl:DatatypeProperty ;
  rdfs:label "URL" ;
  rdfs:comment "The Request URL for this hypermedia." ;
  rdfs:domain hm:HypermediaLink ;
  rdfs:range xsd:string ;
  doc:example """
    @prefix hm: <http://vocab.cosmicdynamo.net/hypermedia.owl#> .
    @prefix ex: <http://example.com/example.owl#> .
    
    @base <http://example.com/> .

    <Object/initial> a hm:Resource ;
      hm:hasLink [ 
        a hm:IdempotentLink ,
          ex:Action ;
        hm:hasMethod hm:Put ;
        hm:url "http://example.com/Object/doSomething"
      ] .
  """ .


#################################################################
#
#    Classes
#
#################################################################

###  http://vocab.cosmicdynamo.net/hypermedia.owl#CreateResourceOperation
hm:CreateResource a owl:Class ;
  rdfs:label "Create Resource" ;
  rdfs:comment "A link that represents a resource creation request" ;
  rdfs:subClassOf hm:NonIdempotentLink , [
    a owl:Restriction ;
    owl:hasValue hm:Post ;
    owl:onProperty hm:hasMethod
  ] , [
    a owl:Restriction ;
    owl:minCardinality "1"^^xsd:nonNegativeInteger ;
    owl:onProperty hm:acceptsResource
  ] , [
    a owl:Restriction ;
    owl:minCardinality "1"^^xsd:nonNegativeInteger ;
    owl:onProperty hm:providesResource
  ] ;
  doc:example """
    @prefix hm: <http://vocab.cosmicdynamo.net/hypermedia.owl#> .                      
    @prefix ex: <http://example.com/example.owl#> .
    
    @base <http://example.com/> .

    <Object/initial> a hm:Resource ,
                       hm:InitialState ;
      hm:hasLink [ 
        a hm:NonIdempotentLink ,
          hm:CreateResource ;
        hm:hasMethod hm:Post ;
        hm:url "http://example.com/Object/" ;
        hm:acceptsResource hm:Resource ;
        hm:providesResource hm:Resource 
      ] .
  """ .

###  http://vocab.cosmicdynamo.net/hypermedia.owl#DeleteResourceOperation
hm:DeleteResource a owl:Class ;
  rdfs:label "Delete Resource" ;
  rdfs:comment "A Delete Resource request" ;
  rdfs:subClassOf hm:IdempotentLink , [
    a owl:Restriction ;
    owl:hasValue hm:Delete ;
    owl:onProperty hm:hasMethod
  ] , [
    a owl:Restriction ;
    owl:maxCardinality "0"^^xsd:nonNegativeInteger ;
    owl:onProperty hm:acceptsResource
  ] , [
    a owl:Restriction ;
    owl:maxCardinality "0"^^xsd:nonNegativeInteger ;
    owl:onProperty hm:providesResource
  ] ;
  doc:example """
    @prefix hm: <http://vocab.cosmicdynamo.net/hypermedia.owl#> .                      
    @prefix ex: <http://example.com/example.owl#> .
    
    @base <http://example.com/> .

    <Object/id/1> a hm:Resource ;
      hm:hasLink [ 
          a hm:NonIdempotentLink ,
            hm:DeleteResource ;
          hm:hasMethod hm:Delete ;
          hm:url "http://example.com/Object/id/1"
      ] .
  """ .

###  http://vocab.cosmicdynamo.net/hypermedia.owl#EmbedLink
hm:EmbedLink a owl:Class ;
  rdfs:label "Embed Link" ;
  rdfs:comment """A Link used to request either update or to request the full representation of the parent Resource.
    NOTE: By convention the IRI of an object should be equivalent to the embed link URL for that object.  This makes sending the Embed Link as a separate Link definition redundant
  """ ;
  rdfs:subClassOf hm:IdempotentLink , [
    a owl:Restriction ;
    owl:hasValue hm:Get ;
    owl:onProperty hm:hasMethod
  ] , [
    a owl:Restriction ;
    owl:maxCardinality "0"^^xsd:nonNegativeInteger ;
    owl:onProperty hm:acceptsResource
  ] , [
    a owl:Restriction ;
    owl:minCardinality "1"^^xsd:nonNegativeInteger ;
    owl:onProperty hm:providesResource
  ] ;
  doc:example """
    @prefix hm: <http://vocab.cosmicdynamo.net/hypermedia.owl#> .                      
    @prefix ex: <http://example.com/example.owl#> .
    
    @base <http://example.com/> .

    <Object/id/1> a hm:Resource ;
      hm:hasLink [ 
        a hm:IdempotentLink ,
          hm:EmbedLink ;
        hm:hasMethod hm:Get ;
        hm:url "http://example.com/Object/id/1"
      ] .
  """ .

###  http://vocab.cosmicdynamo.net/hypermedia.owl#Frame
hm:Frame a owl:Class ;
  rdfs:label "Request Body Frame" ;
  rdfs:comment "Instructions on how to reduce an RDF request body to only triples understood/accepted by the server" ;
  doc:example "Example is not possible for this Object-Type" .

###  http://vocab.cosmicdynamo.net/hypermedia.owl#HttpMethod
hm:HttpMethod a owl:Class ;
  rdfs:label "HTTP Method" ;
  rdfs:comment "The HTTP method that must be used to execute a given Hypermedia Link" ;
  rdfs:subClassOf [
    a owl:Restriction ;
    owl:minCardinality "1"^^xsd:nonNegativeInteger ;
    owl:onProperty http:methodName
  ] , [
    a owl:Restriction ;
    owl:maxCardinality "1"^^xsd:nonNegativeInteger ;
    owl:onProperty http:methodName
  ] ;
  doc:example """
    See:
    http://vocab.cosmicdynamo.net/hypermedia.owl#Delete
    http://vocab.cosmicdynamo.net/hypermedia.owl#Get
    http://vocab.cosmicdynamo.net/hypermedia.owl#Head
    http://vocab.cosmicdynamo.net/hypermedia.owl#Options
    http://vocab.cosmicdynamo.net/hypermedia.owl#Patch
    http://vocab.cosmicdynamo.net/hypermedia.owl#Post
    http://vocab.cosmicdynamo.net/hypermedia.owl#Put
  """ .

###  http://vocab.cosmicdynamo.net/hypermedia.owl#HypermediaLink
hm:HypermediaLink a owl:Class ;
  rdfs:label "Hypermedia Link" ;
  rdfs:comment "An Instruction set telling an RDF client how to perform an action on the parent object which requires a Hypermedia Request to be set to a Semantic Service" ;
  rdfs:subClassOf [
    a owl:Restriction ;
    owl:minCardinality "0"^^xsd:nonNegativeInteger ;
    owl:onProperty hm:acceptsResource
  ] , [
    a owl:Restriction ;
    owl:maxCardinality "1"^^xsd:nonNegativeInteger ;
    owl:onProperty hm:acceptsResource
  ] , [
    a owl:Restriction ;
    owl:minCardinality "1"^^xsd:nonNegativeInteger ;
    owl:onProperty hm:url
  ] , [
    a owl:Restriction ;
    owl:maxCardinality "1"^^xsd:nonNegativeInteger ;
    owl:onProperty hm:url
  ] , [
    a owl:Restriction ;
    owl:minCardinality "1"^^xsd:nonNegativeInteger ;
    owl:onProperty hm:hasMethod
  ] , [
    a owl:Restriction ;
    owl:maxCardinality "1"^^xsd:nonNegativeInteger ;
    owl:onProperty hm:hasMethod
  ] , [
    a owl:Restriction ;
    owl:minCardinality "0"^^xsd:nonNegativeInteger ;
    owl:onProperty hm:providesResource
  ] , [
    a owl:Restriction ;
    owl:maxCardinality "1"^^xsd:nonNegativeInteger ;
    owl:onProperty hm:providesResource
  ] , [
    a owl:Restriction ;
    owl:minCardinality "0"^^xsd:nonNegativeInteger ;
    owl:onProperty hm:useFrame
  ] , [
    a owl:Restriction ;
    owl:maxCardinality "1"^^xsd:nonNegativeInteger ;
    owl:onProperty hm:useFrame
  ] ;
  doc:example """
    @prefix hm: <http://vocab.cosmicdynamo.net/hypermedia.owl#> .                      
    @prefix ex: <http://example.com/example.owl#> .

    @base <http://example.com/> .

    <Object/id/1> a hm:Resource ;
      hm:hasLink [ 
        a hm:HypermediaLink ;
        hm:hasMethod hm:Get ;
        hm:url "http://example.com/Object/id/1"
      ] .
  """ .

###  http://vocab.cosmicdynamo.net/hypermedia.owl#IdempotentLink
hm:IdempotentLink a owl:Class ;
  rdfs:label "Idempotent Link" ;
  rdfs:subClassOf hm:HypermediaLink ;
  rdfs:comment "A link that can be requested multiple times without changing the result beyond the initial application" ;
  doc:example """
    @prefix hm: <http://vocab.cosmicdynamo.net/hypermedia.owl#> .                      
    @prefix ex: <http://example.com/example.owl#> .
    
    @base <http://example.com/> .

    <Object/id/1> a hm:Resource ;
      hm:hasLink [ 
          a hm:IdempotentLink ;
          hm:hasMethod hm:Get ;
          hm:url "http://example.com/Object/id/1"
      ] .
  """ .

###  http://vocab.cosmicdynamo.net/hypermedia.owl#JsonLdFrame
hm:JsonLdFrame a owl:Class ;
    rdfs:label "JSON-LD Frame" ;
    rdfs:subClassOf hm:Frame ;
    rdfs:comment "The assumed type of any JSON-LD Frame document.  See http://json-ld.org/spec/latest/json-ld-framing/ for details on the JSON-LD Framing specification" ;
    doc:example """
        {
          "@context": {
            "ical": "http://www.w3.org/2002/12/cal/ical#",
            "xsd": "http://www.w3.org/2001/XMLSchema#",
            "ical:dtstart": {
              "@type": "xsd:dateTime"
            }
          }
        }
    """ .

###  http://vocab.cosmicdynamo.net/hypermedia.owl#NonIdempotentLink
hm:NonIdempotentLink a owl:Class ;
  rdfs:label "Non-Idempotent Link" ;
  rdfs:subClassOf hm:HypermediaLink ;
  rdfs:comment "A link that CAN NOT be requested multiple times without changing the result beyond the initial application" ;
  doc:example """
    @prefix hm: <http://vocab.cosmicdynamo.net/hypermedia.owl#> .                      
    @prefix ex: <http://example.com/example.owl#> .
    
    @base <http://example.com/> .

    <Object/id/1> a hm:Resource ;
      hm:hasLink [ 
        a hm:NonIdempotentLink ,
          ex:Action ;
        hm:hasMethod hm:Post ;
        hm:url "http://example.com/Object/id/1/doSomething"
      ] .
  """ .

###  http://vocab.cosmicdynamo.net/hypermedia.owl#OutboundLink
hm:OutboundLink rdf:type owl:Class ;
  rdfs:label "Outbound Link" ;
  rdfs:comment "A Request for data that is related, but not bound to it's parent object" ;
  rdfs:subClassOf hm:IdempotentLink , [
    a owl:Restriction ;
    owl:hasValue hm:Get ;
    owl:onProperty hm:hasMethod
  ] , [
    a owl:Restriction ;
    owl:maxCardinality "0"^^xsd:nonNegativeInteger ;
    owl:onProperty hm:acceptsResource
  ] , [
    a owl:Restriction ;
    owl:minCardinality "1"^^xsd:nonNegativeInteger ;
    owl:onProperty hm:providesResource
  ] ;
  doc:example """
    @prefix hm: <http://vocab.cosmicdynamo.net/hypermedia.owl#> .                      
    @prefix ex: <http://example.com/example.owl#> .
    
    @base <http://example.com/> .

    <Object/id/1> a hm:Resource ;
      hm:hasLink [ 
        a hm:OutboundLink ;
        hm:hasMethod hm:Get ;
        hm:url "http://example.com/Object/id/1"
      ] .
  """ .


###  http://vocab.cosmicdynamo.net/hypermedia.owl#ReplaceResourceOperation
hm:ReplaceResource rdf:type owl:Class ;
  rdfs:label "Replace Resource" ;
  rdfs:subClassOf hm:IdempotentLink , [
    a owl:Restriction ;
    owl:hasValue hm:Put ;
    owl:onProperty hm:hasMethod
  ] , [
    a owl:Restriction ;
    owl:minCardinality "1"^^xsd:nonNegativeInteger ;
    owl:onProperty hm:acceptsResource
  ] , [
    a owl:Restriction ;
    owl:minCardinality "1"^^xsd:nonNegativeInteger ;
    owl:onProperty hm:providesResource
  ] ;
  rdfs:comment "A request that will replace the existing resource with the request body" ;
  doc:example """
    @prefix hm: <http://vocab.cosmicdynamo.net/hypermedia.owl#> .                      
    @prefix ex: <http://example.com/example.owl#> .
    
    @base <http://example.com/> .

    <Object/id/1> a hm:Resource ;
      hm:hasLink [ 
        a hm:NonIdempotentLink ,
          hm:ReplaceResource ;
        hm:hasMethod hm:Put ;
        hm:url "http://example.com/Object/id/1/doSomething" ;
        hm:acceptsResource hm:Resource ;
        hm:providesResource hm:Resource
      ] .
  """ .

###  http://vocab.cosmicdynamo.net/hypermedia.owl#SourceDataLink
hm:SourceDataLink a owl:Class ;
  rdfs:label "Source Data Link" ;
  rdfs:subClassOf hm:OutboundLink , [
    a owl:Restriction ;
    owl:minCardinality "1"^^xsd:nonNegativeInteger ;
    owl:onProperty hm:dataPredicate;
  ] , [
    a owl:Restriction ;
    owl:maxCardinality "1"^^xsd:nonNegativeInteger ;
    owl:onProperty hm:dataPredicate;
  ] ;
  rdfs:comment "Hypermedia Link which provides information about allowed values for a given data predicate on the parent Hypermedia Resource" ;
  doc:example """
    @prefix hm: <http://vocab.cosmicdynamo.net/hypermedia.owl#> .
    @prefix ex: <http://example.com/example.owl#> .
    
    @base <http://example.com/> .

    <Object/initial> a hm:Resource ;
      ex:hasField <Enumeration/000> ;
      hm:hasLink [ 
        a hm:IdempotentLink ,
          hm:SourceDataLink ;
        hm:hasMethod hm:Get ;
        hm:url "http://example.com/Enumeration" ;
        hm:providesResource ex:EnumeratedType ;
        hm:dataPredicate ex:hasField
      ] .
  """ .

###  http://vocab.cosmicdynamo.net/hypermedia.owl#InitialStateLink
hm:InitialStateLink a owl:Class ;
  rdfs:label "Initial State Link" ;
  rdfs:comment "Provides a Link to a Representation of the Default State of a New Object created for the Collection which contains this link" ;
  rdfs:subClassOf hm:OutboundLink ;
  doc:example """
    @prefix hm: <http://vocab.cosmicdynamo.net/hypermedia.owl#> .
    @prefix col: <http://vocab.cosmicdynamo.net/collection.owl#> .
    @prefix ex: <http://vocab.example.com/example.owl#> .
    
    @prefix xsd: <http://www.w3.org/2001/XMLSchema#> .

    @base <http://example.com/Object/1/> .

    <> a ex:ObjectCollection .

    <Children/> a col:Container ;
      col:membershipSubject <> ;
      col:membershipPredicate ex:hasChildren ;
      col:totalCount "0"^^xsd:nonNegativeInteger ;
      hm:hasLink [
        a hm:OutboundLink ,
          hm:InitialStateLink ;
          hm:method hm:Get ;
          hm:url "http://example.com/Object/1/Children/new" ;
          hm:providesResource ex:ChildType
      ] .
  """ .
                    
hm:InitialStateCollection a owl:Class ;
  rdfs:label "Collection Of Initial State Objects" ;
  rdfs:comment "A collection of Initial State Object which meet some search criteria" ;
  rdfs:subClassOf [
    a owl:Restriction ;
    owl:onProperty hm:hasLink ;
    owl:minCardinality "0"^^xsd:nonNegativeInteger 
  ] ;
  doc:example """
    @prefix hm: <http://vocab.cosmicdynamo.net/hypermedia.owl#> .
    @prefix col: <http://vocab.cosmicdynamo.net/collection.owl#> .
    @prefix ex: <http://vocab.example.com/example.owl#> .

    @prefix xsd: <http://www.w3.org/2001/XMLSchema#> .
    
    @base <http://example.com/Object/1/Children/new> .

    <?type=http://example.com/SubType1> a hm:InitialStateCollection ;
      hm:hasLink [
        a hm:OutboundLink ,
          hm:InitialStateLink ;
        hm:method hm:Get ;
        hm:url "http://example.com/Object/1/Children/new/SubType1" ;
        hm:providesResource ex:SubType1
      ].

    <?type=http://example.com/SubType1> a col:Container , 
                                          col:SearchResult ;
      hm:membershipSubject <?type=http://example.com/SubType1> ;
      hm:hasSourceContainer <?type=all> ;
      hm:membershipPredicate hm:hasLink ;
      hm:totalCount "1"^^xsd:nonNegativeInteger .
  """ .

###  http://vocab.cosmicdynamo.net/hypermedia.owl#TemplateItem
hm:TemplateItem a owl:Class ;
  rdfs:label "Template Item" ;
  rdfs:comment "A template item represents a template parameter to be set by the client as part of a template link." ;
  rdfs:subClassOf [
    a owl:Restriction ;
    owl:minCardinality "1"^^xsd:nonNegativeInteger ;
    owl:onProperty hm:templateItemPredicate
  ] , [
    a owl:Restriction ;
    owl:maxCardinality "1"^^xsd:nonNegativeInteger ;
    owl:onProperty hm:templateItemPredicate
  ] ,  [
    a owl:Restriction ;
    owl:minCardinality "1"^^xsd:nonNegativeInteger ;
    owl:onProperty hm:token
  ] , [
    a owl:Restriction ;
    owl:maxCardinality "1"^^xsd:nonNegativeInteger ;
    owl:onProperty hm:token
  ] ;
  doc:example """
    @prefix hm: <http://vocab.cosmicdynamo.net/hypermedia.owl#> .
    @prefix ex: <http://example.com/example.owl#> .
    
    <Object/id/1> a hm:Resource ;
      ex:field "value" ;
      hm:hasLink [
        a hm:TemplateLink ,
          ex:Action ;
        hm:templateUrl "http://example.com/Object/id/1/doSomething?param={value}" ;
        hm:hasMethod hm:Put ;
        hm:hasTemplateItem [
          hm:token "{value}" ;
          hm:templateItemPredicate ex:field 
        ]
      ] .
  """ .

###  http://vocab.cosmicdynamo.net/hypermedia.owl#TemplateLink
hm:TemplateLink a owl:Class ;
  rdfs:label "Template Link" ;
  rdfs:subClassOf hm:HypermediaLink ;
  rdfs:comment "A Link that MUST be constructed using a template string with tokens that can be replaced at runtime to form a valid URL" ;
  rdfs:subClassOf [
    a owl:Restriction ;
    owl:minCardinality "1"^^xsd:nonNegativeInteger ;
    owl:onProperty hm:hasTemplateItem
  ] ,  [
    a owl:Restriction ;
    owl:minCardinality "1"^^xsd:nonNegativeInteger ;
    owl:onProperty hm:templateUrl
  ] ,  [
    a owl:Restriction ;
    owl:maxCardinality "1"^^xsd:nonNegativeInteger ;
    owl:onProperty hm:templateUrl
  ] , [
    a owl:Restriction ;
    owl:maxCardinality "0"^^xsd:nonNegativeInteger ;
    owl:onProperty hm:url
  ] , [
    a owl:Restriction ;
    owl:hasValue hm:Get ;
    owl:onProperty hm:hasMethod
  ] ;
  doc:example """
    @prefix hm: <http://vocab.cosmicdynamo.net/hypermedia.owl#> .
    @prefix ex: <http://example.com/example.owl#> .

    <Object/id/1> a hm:Resource ;
      ex:field "value" ;
      hm:hasLink [
        a hm:TemplateLink ,
          ex:Action ;
        hm:templateUrl "http://example.com/Object/id/1/doSomething?param={value}" ;
        hm:hasMethod hm:Put ;
        hm:hasTemplateItem [
          hm:token "{value}" ;
          hm:templateItemPredicate ex:field 
        ]
      ] .
  """ .

###  http://vocab.cosmicdynamo.net/hypermedia.owl#Resource
hm:ResourceDescription a rdfs:Class ;
  rdfs:label "Resource Description" ;
  rdfs:comment "Details about how to find and interact with a given resource type" ;
  rdfs:subClassOf hm:Resource , [
    a owl:Restriction ;
    owl:minCardinality "1"^^xsd:nonNegativeInteger ;
    owl:onProperty hm:hasOntology
  ] , [
    a owl:Restriction ;
    owl:maxCardinality "1"^^xsd:nonNegativeInteger ;
    owl:onProperty hm:hasOntology
  ] , [
    a owl:Restriction ;
    owl:minCardinality "1"^^xsd:nonNegativeInteger ;
    owl:onProperty hm:serves
  ] , [
    a owl:Restriction ;
    owl:maxCardinality "1"^^xsd:nonNegativeInteger ;
    owl:onProperty hm:serves
  ] ;
  doc:example """
    @prefix ex: <http://example.com/example.owl#> .
    @prefix hm: <http://vocab.cosmicdynamo.net/hypermedia.owl#> .
    @prefix col: <http://vocab.cosmicdynamo.net/collection.owl#> .
    
    @prefix xsd: <http://www.w3.org/2001/XMLSchema#> .

    @base <http://example.com/api/> .

    <> a hm:ResourceDiscoveryDocument;
      hm:hasResource ( <ObjectType> ) .

    <?typeiri=http%3A%2F%2Fvocab.example.com%2F2014%example.owl%23ObjectType> a col:SearchResult, 
                                                                                col:Container;
      col:membershipSubject <> ;
      col:membershipPredicate hm:hasResource ;
      col:totalCount "1"^^xsd:nonNegativeInteger .
        
    <ObjectType> a hm:ResourceDescription ;
      hm:hasOntology <ObjectType/ontology> ;
      hm:serves ex:ObjectType .
    """ .

###  http://vocab.cosmicdynamo.net/hypermedia.owl#ResourceDiscoveryDocument
hm:ResourceDiscoveryDocument a owl:Class ;
  rdfs:label "Resource Discovery Document" ;
  rdfs:comment "A Container for top-level resource information;  Can be either a collection of all Resources exposed by a Service or a sub-set matching some Search criteria" ;
  rdfs:subClassOf [
    a owl:Restriction ;
    owl:minCardinality "0"^^xsd:nonNegativeInteger ;
    owl:onProperty hm:hasResource
  ] ;
  doc:example """
    @prefix ex: <http://example.com/example.owl#> .
    @prefix hm: <http://vocab.cosmicdynamo.net/hypermedia.owl#> .
    @prefix col: <http://vocab.cosmicdynamo.net/collection.owl#> .
    
    @prefix xsd: <http://www.w3.org/2001/XMLSchema#> .

    @base <http://example.com/api/> .

    <> a hm:ResourceDiscoveryDocument;
       hm:hasResource ( <ObjectType> ) .

    <?typeiri=http%3A%2F%2Fvocab.example.com%2F2014%example.owl%23ObjectType> a col:SearchResult, 
                                                                                col:Container;
      col:membershipSubject <> ;
      col:membershipPredicate hm:hasResource ;
      col:totalCount "1"^^xsd:nonNegativeInteger .
        
    <ObjectType> a hm:ResourceDescription ;
      hm:hasOntology <ObjectType/ontology> ;
      hm:serves ex:ObjectType .
    """ .

###  http://vocab.cosmicdynamo.net/hypermedia.owl#ResourceDiscoveryDocument
hm:Resource a owl:Class ;
  rdfs:label "Hypermedia Resource" ;
  rdfs:comment "An object which contains Hypermedia Links" ;
  rdfs:subClassOf [
  a owl:Restriction ;
    owl:minCardinality "0"^^xsd:nonNegativeInteger ;
    owl:onProperty hm:hasLink
  ] ;
  doc:example """
    @prefix hm: <http://vocab.cosmicdynamo.net/hypermedia.owl#> .
    @prefix ex: <http://example.com/example.owl#> .
    
    <Object/id/1> a hm:Resource ;
      ex:field "value" ;
      hm:hasLink [
        a hm:IdempotentLink ,
          ex:Action ;
        hm:url "http://example.com/Object/id/1/doSomething" ;
        hm:hasMethod hm:Get
      ] .
  """ .


#################################################################
#
#    Individuals
#
#################################################################

###  http://vocab.cosmicdynamo.net/hypermedia.owl#Delete
hm:Delete rdf:type hm:HttpMethod ,
                   owl:NamedIndividual ;
  rdfs:label "Delete" ;
  http:methodName "DELETE"^^xsd:string ;
  rdfs:comment "HTTP DELETE method instance." ;
  doc:example """
    @prefix hm: <http://vocab.cosmicdynamo.net/hypermedia.owl#> .                      
    @prefix ex: <http://example.com/example.owl#> .
    
    @base <http://example.com/> .

    <Object/id/1> a hm:Resource ;
      hm:hasLink [ 
        a hm:NonIdempotentLink ,
          hm:DeleteResource ;
        hm:hasMethod hm:Delete ;
        hm:url "http://example.com/Object/id/1"
      ] .
  """ .

###  http://vocab.cosmicdynamo.net/hypermedia.owl#Get
hm:Get a hm:HttpMethod ,
         owl:NamedIndividual ;
  rdfs:label "Get" ;
  http:methodName "GET" ;
  rdfs:comment "HTTP GET method instance." ;
  doc:example """
    @prefix hm: <http://vocab.cosmicdynamo.net/hypermedia.owl#> .
    @prefix ex: <http://example.com/example.owl#> .
    
    @base <http://example.com/> .

    <Object/id/0> a hm:Resource ;
      hm:hasLink  [ 
        a hm:IdempotentLink ,
          ex:Action ;
        hm:hasMethod hm:Get ;
        hm:url "http://example.com/Object/details" ;
        hm:providesResource ex:ChildThing
      ] .
  """ .

###  http://vocab.cosmicdynamo.net/hypermedia.owl#Head
hm:Head a hm:HttpMethod ,
          owl:NamedIndividual ;
  rdfs:label "Head" ;
  http:methodName "HEAD"^^xsd:string ;
  rdfs:comment "HTTP HEAD method instance." ;
  doc:example "This instance is here for completeness;  There are currently no known Use Cases to expose a HEAD Link to a client" .

###  http://vocab.cosmicdynamo.net/hypermedia.owl#Options
hm:Options a hm:HttpMethod ,
             owl:NamedIndividual ;
  rdfs:label "Options" ;
  http:methodName "OPTIONS"^^xsd:string ;
  rdfs:comment "HTTP OPTIONS method instance." ;
  doc:example "This instance is here for completeness;  There are currently no known Use Cases to expose a OPTIONAL Link to a client" .

###  http://vocab.cosmicdynamo.net/hypermedia.owl#Patch
hm:Patch a hm:HttpMethod ,
           owl:NamedIndividual ;
  rdfs:label "Patch" ;
  http:methodName "PATCH"^^xsd:string ;
  rdfs:comment "HTTP PATCH method instance."  ;
  doc:example """
    @prefix hm: <http://vocab.cosmicdynamo.net/hypermedia.owl#> .
    @prefix ex: <http://example.com/example.owl#> .
    
    @base <http://example.com/> .

    <Object/id/001> a hm:Resource ;
      hm:hasLink [ 
          a hm:IdempotentLink ,
            ex:Action ;
          hm:hasMethod hm:Patch ;
          hm:url "http://example.com/Object/id/001" ;
          hm:acceptsResource ex:NonPersonalClient
      ] .
  """ .

###  http://vocab.cosmicdynamo.net/hypermedia.owl#Post
hm:Post a hm:HttpMethod ,
          owl:NamedIndividual ;
  rdfs:label "Post" ;
  http:methodName "POST"^^xsd:string ;
  rdfs:comment "HTTP POST method instance."  ;
  doc:example """
    @prefix hm: <http://vocab.cosmicdynamo.net/hypermedia.owl#> .
    @prefix ex: <http://example.com/example.owl#> .
    
    @base <http://example.com/> .

    <Object/initial> a hm:Resource ,
                       hm:InitialState ;
      hm:hasLink [ 
        a hm:IdempotentLink ,
          ex:Action ;
        hm:hasMethod hm:Post ;
        hm:url "http://example.com/Object" ;
        hm:acceptsResource ex:NonPersonalClient
      ] .
  """ .

###  http://vocab.cosmicdynamo.net/hypermedia.owl#Put
hm:Put a hm:HttpMethod ,
         owl:NamedIndividual ;
  rdfs:label "Put" ;
  http:methodName "PUT"^^xsd:string ;
  rdfs:comment "HTTP PUT method instance."  ;
  doc:example """
    @prefix hm: <http://vocab.cosmicdynamo.net/hypermedia.owl#> .
    @prefix ex: <http://example.com/example.owl#> .
    
    @base <http://example.com/> .

    <Object/id/001> a hm:Resource ;
      hm:hasLink [ 
        a hm:IdempotentLink ,
          ex:Action ;
        hm:hasMethod hm:Put ;
        hm:url "http://example.com/Object/id/001" ;
        hm:acceptsResource ex:NonPersonalClient
      ] .
  """ .
